r2XSP_RTEP.v
@@ -27,274 +27,414 @@ Hypothesis tgt_sem           : semantics_safety_like tgt.
 (*   end.  *)
 
 
-Fixpoint list_pref { A : Type } (l1 l2 : list A) : Prop :=
-  match l1, l2 with
-  | nil, _ => True
-  | cons x xs, cons y ys => x = y /\ list_pref xs ys
-  | _, _ => False
-  end.
+(* Fixpoint list_pref { A : Type } (l1 l2 : list A) : Prop := *)
+(*   match l1, l2 with *)
+(*   | nil, _ => True *)
+(*   | cons x xs, cons y ys => x = y /\ list_pref xs ys *)
+(*   | _, _ => False *)
+(*   end. *)
 
-Fixpoint list_pref_trace (l : list event) (t : trace) : Prop :=
-  match l with  
-  | nil => True
-  | cons x xs => match t with
-                | tcons e t' => x = e /\ list_pref_trace xs t'
-                | _ => False
-                end
-  end. 
+(* Fixpoint list_pref_trace (l : list event) (t : trace) : Prop := *)
+(*   match l with   *)
+(*   | nil => True *)
+(*   | cons x xs => match t with *)
+(*                 | tcons e t' => x = e /\ list_pref_trace xs t' *)
+(*                 | _ => False *)
+(*                 end *)
+(*   end.  *)
 
     
-Definition xpr (x1 x2 : xpref) : Prop :=
-  match x1 with
-  | xstop m1 s1 => match x2 with
-                  | xstop m2 s2 => m1 = m2 /\ s1 = s2
-                  | _ => False
-                  end
+(* Definition xpr (x1 x2 : xpref) : Prop := *)
+(*   match x1 with *)
+(*   | xstop m1 s1 => match x2 with *)
+(*                   | xstop m2 s2 => m1 = m2 /\ s1 = s2 *)
+(*                   | _ => False *)
+(*                   end *)
                     
-  | xsilent m1 => match x2 with
-                 | xsilent m2 => m1 = m2
-                 | _ => False
-                 end
+(*   | xsilent m1 => match x2 with *)
+(*                  | xsilent m2 => m1 = m2 *)
+(*                  | _ => False *)
+(*                  end *)
                    
-  | xtbd m1 => match x2 with
-              | xstop m2 s1 => list_pref m1 m2
-              | xsilent m2  => list_pref m1 m2
-              | xtbd m2 =>  list_pref m1 m2
-              end
+(*   | xtbd m1 => match x2 with *)
+(*               | xstop m2 s1 => list_pref m1 m2 *)
+(*               | xsilent m2  => list_pref m1 m2 *)
+(*               | xtbd m2 =>  list_pref m1 m2 *)
+(*               end *)
                 
-  end.
+(*   end. *)
 
-Definition xstopped x : bool :=
-  match x with
-  | xstop _ _ => true
-  | _ => false
-  end.
+(* Definition xstopped x : bool := *)
+(*   match x with *)
+(*   | xstop _ _ => true *)
+(*   | _ => false *)
+(*   end. *)
 
-Lemma xpr_snoc : forall p a1 a2, 
-    xpr (xtbd (snoc p a1)) (xtbd (snoc p a2)) -> a1 = a2.
-Proof.
-  induction p; intros a1 a2 H; simpl in *; destruct H as [H1 H2]; auto.   
-Qed.
+(* Lemma xpr_snoc : forall p a1 a2,  *)
+(*     xpr (xtbd (snoc p a1)) (xtbd (snoc p a2)) -> a1 = a2. *)
+(* Proof. *)
+(*   induction p; intros a1 a2 H; simpl in *; destruct H as [H1 H2]; auto.    *)
+(* Qed. *)
 
-Fixpoint list_to_stop_trace (l : list event) (e : endstate) : trace :=
-  match l with
-  | nil => tstop e
-  | cons l ls => tcons l (list_to_stop_trace ls e)
-  end. 
+(* Fixpoint list_to_stop_trace (l : list event) (e : endstate) : trace := *)
+(*   match l with *)
+(*   | nil => tstop e *)
+(*   | cons l ls => tcons l (list_to_stop_trace ls e) *)
+(*   end.  *)
 
-Lemma xstop_prefix_list : forall p e, xprefix (xstop p e) (list_to_stop_trace p e).
-Proof.
-  induction p; intros e; simpl; auto.  
-  split; auto. now apply IHp.
-Qed.
+(* Lemma xstop_prefix_list : forall p e, xprefix (xstop p e) (list_to_stop_trace p e). *)
+(* Proof. *)
+(*   induction p; intros e; simpl; auto.   *)
+(*   split; auto. now apply IHp. *)
+(* Qed. *)
 
-Lemma unique_continuation_stop: forall l e t, xprefix (xstop l e) t -> t = list_to_stop_trace l e. 
-Proof.
-  intros l e. induction l.
-  + intros [] Hxpref; auto; inversion Hxpref; now subst. 
-  + intros [] Hxpref; inversion Hxpref. subst. 
-    simpl. now rewrite (IHl t).    
-Qed.
+(* Lemma unique_continuation_stop: forall l e t, xprefix (xstop l e) t -> t = list_to_stop_trace l e.  *)
+(* Proof. *)
+(*   intros l e. induction l. *)
+(*   + intros [] Hxpref; auto; inversion Hxpref; now subst.  *)
+(*   + intros [] Hxpref; inversion Hxpref. subst.  *)
+(*     simpl. now rewrite (IHl t).     *)
+(* Qed. *)
 
-Fixpoint list_to_silent_trace (l : list event) : trace :=
-  match l with
-  | nil => tsilent
-  | cons l ls => tcons l (list_to_silent_trace ls)
-  end.
+(* Fixpoint list_to_silent_trace (l : list event) : trace := *)
+(*   match l with *)
+(*   | nil => tsilent *)
+(*   | cons l ls => tcons l (list_to_silent_trace ls) *)
+(*   end. *)
 
-Lemma xsilent_prefix_list : forall p, xprefix (xsilent p) (list_to_silent_trace p).
-Proof.
-  induction p; simpl; auto.  
-Qed.
+(* Lemma xsilent_prefix_list : forall p, xprefix (xsilent p) (list_to_silent_trace p). *)
+(* Proof. *)
+(*   induction p; simpl; auto.   *)
+(* Qed. *)
 
-Lemma unique_continuation_silent : forall l t, xprefix (xsilent l) t -> t = list_to_silent_trace l.
-Proof.  
-   intros l. induction l; intros [] Hxpref; auto; inversion Hxpref; subst. 
-   simpl. now rewrite (IHl t).    
-Qed. 
+(* Lemma unique_continuation_silent : forall l t, xprefix (xsilent l) t -> t = list_to_silent_trace l. *)
+(* Proof.   *)
+(*    intros l. induction l; intros [] Hxpref; auto; inversion Hxpref; subst.  *)
+(*    simpl. now rewrite (IHl t).     *)
+(* Qed.  *)
   
-Lemma three_continuations_tbd :
-  forall l t, xprefix (xtbd l) t ->
-         ( (exists e, t = list_to_stop_trace l e) \/                                     
-                 (t = list_to_silent_trace l) \/
-            (exists e, xprefix (xtbd (snoc l e)) t)). 
-Proof.
-  intros l. induction l.
-  + intros [] Hxpref.
-    ++ left. now exists e.
-    ++ right. now left.
-    ++ right. right. now exists e.
-  + intros [] Hxpref; inversion Hxpref; subst.
-    destruct  (IHl t) as [K1 | [K2 | K3]]; auto.  
-    ++ left. destruct K1 as [e0 K1]. exists e0. simpl. now rewrite K1.
-    ++ right. left. simpl. now rewrite K2.
-    ++ right. right. destruct K3 as [e0 K3]. now exists e0.
-Qed.
+(* Lemma three_continuations_tbd : *)
+(*   forall l t, xprefix (xtbd l) t -> *)
+(*          ( (exists e, t = list_to_stop_trace l e) \/                                      *)
+(*                  (t = list_to_silent_trace l) \/ *)
+(*             (exists e, xprefix (xtbd (snoc l e)) t)).  *)
+(* Proof. *)
+(*   intros l. induction l. *)
+(*   + intros [] Hxpref. *)
+(*     ++ left. now exists e. *)
+(*     ++ right. now left. *)
+(*     ++ right. right. now exists e. *)
+(*   + intros [] Hxpref; inversion Hxpref; subst. *)
+(*     destruct  (IHl t) as [K1 | [K2 | K3]]; auto.   *)
+(*     ++ left. destruct K1 as [e0 K1]. exists e0. simpl. now rewrite K1. *)
+(*     ++ right. left. simpl. now rewrite K2. *)
+(*     ++ right. right. destruct K3 as [e0 K3]. now exists e0. *)
+(* Qed. *)
 
-Lemma xpr_longer_stop_contra : forall p a e, xpr (xtbd (snoc p a)) (xstop p e) -> False.
-Proof.
-  induction p; auto.
-  simpl. intros a0 e [Hfoo H]. now apply (IHp a0 e). 
-Qed.
+(* Lemma xpr_longer_stop_contra : forall p a e, xpr (xtbd (snoc p a)) (xstop p e) -> False. *)
+(* Proof. *)
+(*   induction p; auto. *)
+(*   simpl. intros a0 e [Hfoo H]. now apply (IHp a0 e).  *)
+(* Qed. *)
 
-Lemma xpr_longer_silent_contra : forall p a, xpr (xtbd (snoc p a)) (xsilent p) -> False.
-Proof.
-  induction p; auto.
-  simpl. intros a0 [Hfoo H]. now apply (IHp a0).
-Qed. 
+(* Lemma xpr_longer_silent_contra : forall p a, xpr (xtbd (snoc p a)) (xsilent p) -> False. *)
+(* Proof. *)
+(*   induction p; auto. *)
+(*   simpl. intros a0 [Hfoo H]. now apply (IHp a0). *)
+(* Qed.  *)
 
-Lemma xpr_longer_xtbd_contra: forall p a, xpr (xtbd (snoc p a)) (xtbd p) -> False.
-Proof.
-  induction p; auto.
-  simpl. intros a0 [Hfoo H]. now apply (IHp a0).
-Qed. 
+(* Lemma xpr_longer_xtbd_contra: forall p a, xpr (xtbd (snoc p a)) (xtbd p) -> False. *)
+(* Proof. *)
+(*   induction p; auto. *)
+(*   simpl. intros a0 [Hfoo H]. now apply (IHp a0). *)
+(* Qed.  *)
 
-Lemma list_snoc_pointwise: forall (l p : list event) i1 i2 a1 a2,
-                          i1 <> i2 ->
-                          list_pref (snoc l i1) (snoc p a1) ->
-                          list_pref (snoc l i2) (snoc p a2) ->
-                          (i1 = a1 /\ i2 = a2).
-Proof.
-  induction l; intros p i1 i2 a1 a2 diff_i l1_pref l2_pref.
-  + destruct p; inversion l1_pref; inversion l2_pref; auto. 
-    subst. exfalso. now apply diff_i.
-  + destruct p; simpl in l1_pref, l2_pref.
-    ++ destruct l1_pref as [aa1 contra].
-       now destruct l.
-    ++ destruct l1_pref as [ae l1_pref]. destruct l2_pref as [foo l2_pref].
-       now apply (IHl p i1 i2 a1 a2).
-Qed.   
+(* Lemma list_snoc_pointwise: forall (l p : list event) i1 i2 a1 a2, *)
+(*                           i1 <> i2 -> *)
+(*                           list_pref (snoc l i1) (snoc p a1) -> *)
+(*                           list_pref (snoc l i2) (snoc p a2) -> *)
+(*                           (i1 = a1 /\ i2 = a2). *)
+(* Proof. *)
+(*   induction l; intros p i1 i2 a1 a2 diff_i l1_pref l2_pref. *)
+(*   + destruct p; inversion l1_pref; inversion l2_pref; auto.  *)
+(*     subst. exfalso. now apply diff_i. *)
+(*   + destruct p; simpl in l1_pref, l2_pref. *)
+(*     ++ destruct l1_pref as [aa1 contra]. *)
+(*        now destruct l. *)
+(*     ++ destruct l1_pref as [ae l1_pref]. destruct l2_pref as [foo l2_pref]. *)
+(*        now apply (IHl p i1 i2 a1 a2). *)
+(* Qed.    *)
 
-Lemma no_silent_and_stop: forall l1 l2 e,
-    list_to_silent_trace l1 <> list_to_stop_trace l2 e.
-Proof.  
-  intros l. induction l; intros []; try now auto. 
-  + intros e1. intros Hf. inversion Hf.
-    apply ((IHl l0 e1) H1).
-Qed.    
+(* Lemma no_silent_and_stop: forall l1 l2 e, *)
+(*     list_to_silent_trace l1 <> list_to_stop_trace l2 e. *)
+(* Proof.   *)
+(*   intros l. induction l; intros []; try now auto.  *)
+(*   + intros e1. intros Hf. inversion Hf. *)
+(*     apply ((IHl l0 e1) H1). *)
+(* Qed.     *)
 
-Lemma list_same_ext : forall l1 l2 t,
-    list_pref_trace l1 t ->
-    list_pref_trace l2 t ->
-    list_pref l1 l2 \/ list_pref l2 l1.
-Proof.
-  induction l1; intros l2 t H1 H2.
-  + now left.
-  + destruct l2.
-    ++ now right.
-    ++ destruct t; inversion H1; inversion H2; subst.
-       simpl. destruct (IHl1 l2 t); auto. 
-Qed. 
+(* Lemma list_same_ext : forall l1 l2 t, *)
+(*     list_pref_trace l1 t -> *)
+(*     list_pref_trace l2 t -> *)
+(*     list_pref l1 l2 \/ list_pref l2 l1. *)
+(* Proof. *)
+(*   induction l1; intros l2 t H1 H2. *)
+(*   + now left. *)
+(*   + destruct l2. *)
+(*     ++ now right. *)
+(*     ++ destruct t; inversion H1; inversion H2; subst. *)
+(*        simpl. destruct (IHl1 l2 t); auto.  *)
+(* Qed.  *)
 
-Lemma xsilent_prefix_xftbd_prefix : forall p t,
-    xprefix (xsilent p) t -> xprefix (xtbd p) t. 
-Proof.
-  induction p; intros t H; try now auto.  
-  destruct t; inversion H; subst. simpl.
-  split; auto. now apply (IHp t). 
-Qed.
+(* Lemma xsilent_prefix_xftbd_prefix : forall p t, *)
+(*     xprefix (xsilent p) t -> xprefix (xtbd p) t.  *)
+(* Proof. *)
+(*   induction p; intros t H; try now auto.   *)
+(*   destruct t; inversion H; subst. simpl. *)
+(*   split; auto. now apply (IHp t).  *)
+(* Qed. *)
 
-Lemma same_x_ext : forall x1 x2 t, xprefix x1 t -> xprefix x2 t -> xpr x1 x2 \/ xpr x2 x1. 
-Proof.
-  intros []; induction p; intros x2 t H1 H2. 
-  + apply unique_continuation_stop in H1. subst.
-    destruct x2.
-    ++ destruct p. simpl in H2. subst. now left.
-       simpl in *. contradiction.
-    ++ destruct p. simpl in H2. subst. now right.
-       simpl in *. contradiction.
-    ++ destruct p. simpl in H2. contradiction.
-       simpl in *. contradiction.
-  + destruct t; simpl in H1; try contradiction. 
-    inversion H1. subst.
-    destruct x2.
-    ++ destruct p0; simpl in H2. contradiction.
-       inversion H2. subst.
-       destruct (IHp (xstop p0 e1) t) as [K1 | K2]; auto. 
-       +++ left. subst. simpl in *. firstorder. now rewrite H.
-       +++ right. simpl in *. firstorder. now rewrite H.
-    ++ destruct p0; simpl in H2. now right. 
-       destruct (IHp (xtbd p0) t) as [K1 | K2]; auto. 
-       +++ simpl. now destruct H2.  
-       +++ right. simpl. firstorder.
-    ++ apply unique_continuation_silent in H2. 
-       apply unique_continuation_stop in H0.
-       destruct p0; inversion H2.  
-       rewrite H0 in H4. exfalso. symmetry in H4.
-       now apply no_silent_and_stop in H4.     
-  + left. now case x2.
-  + destruct t; inversion H1; subst.
-    destruct x2; simpl in H2.
-    ++ destruct p0; inversion H2; subst.
-       simpl. destruct (IHp (xstop p0 e0) t); auto. 
-    ++ destruct p0; inversion H2; subst.
-       simpl. now right.
-       simpl. destruct (IHp (xtbd p0) t); auto. 
-    ++ admit.
-  + destruct t; try now auto.
-    destruct x2; simpl in  H2; 
-    destruct p; try now auto.
-    now left.  
-  + admit.    
-Admitted.
+(* Lemma same_x_ext : forall x1 x2 t, xprefix x1 t -> xprefix x2 t -> xpr x1 x2 \/ xpr x2 x1.  *)
+(* Proof. *)
+(*   intros []; induction p; intros x2 t H1 H2.  *)
+(*   + apply unique_continuation_stop in H1. subst. *)
+(*     destruct x2. *)
+(*     ++ destruct p. simpl in H2. subst. now left. *)
+(*        simpl in *. contradiction. *)
+(*     ++ destruct p. simpl in H2. subst. now right. *)
+(*        simpl in *. contradiction. *)
+(*     ++ destruct p. simpl in H2. contradiction. *)
+(*        simpl in *. contradiction. *)
+(*   + destruct t; simpl in H1; try contradiction.  *)
+(*     inversion H1. subst. *)
+(*     destruct x2. *)
+(*     ++ destruct p0; simpl in H2. contradiction. *)
+(*        inversion H2. subst. *)
+(*        destruct (IHp (xstop p0 e1) t) as [K1 | K2]; auto.  *)
+(*        +++ left. subst. simpl in *. firstorder. now rewrite H. *)
+(*        +++ right. simpl in *. firstorder. now rewrite H. *)
+(*     ++ destruct p0; simpl in H2. now right.  *)
+(*        destruct (IHp (xtbd p0) t) as [K1 | K2]; auto.  *)
+(*        +++ simpl. now destruct H2.   *)
+(*        +++ right. simpl. firstorder. *)
+(*     ++ apply unique_continuation_silent in H2.  *)
+(*        apply unique_continuation_stop in H0. *)
+(*        destruct p0; inversion H2.   *)
+(*        rewrite H0 in H4. exfalso. symmetry in H4. *)
+(*        now apply no_silent_and_stop in H4.      *)
+(*   + left. now case x2. *)
+(*   + destruct t; inversion H1; subst. *)
+(*     destruct x2; simpl in H2. *)
+(*     ++ destruct p0; inversion H2; subst. *)
+(*        simpl. destruct (IHp (xstop p0 e0) t); auto.  *)
+(*     ++ destruct p0; inversion H2; subst. *)
+(*        simpl. now right. *)
+(*        simpl. destruct (IHp (xtbd p0) t); auto.  *)
+(*     ++ admit. *)
+(*   + destruct t; try now auto. *)
+(*     destruct x2; simpl in  H2;  *)
+(*     destruct p; try now auto. *)
+(*     now left.   *)
+(*   + admit.     *)
+(* Admitted. *)
 
 
-Lemma ftbd_prefix_stop_sublist: forall l p e, ftbd_prefix l (list_to_stop_trace p e) -> list_pref l p. 
-Proof.
-  induction l; intros p e Hpref; auto.
-  destruct p; inversion Hpref.
-  subst. simpl. split; auto. now apply (IHl p e). 
-Qed.
+(* Lemma ftbd_prefix_stop_sublist: forall l p e, ftbd_prefix l (list_to_stop_trace p e) -> list_pref l p.  *)
+(* Proof. *)
+(*   induction l; intros p e Hpref; auto. *)
+(*   destruct p; inversion Hpref. *)
+(*   subst. simpl. split; auto. now apply (IHl p e).  *)
+(* Qed. *)
 
-Lemma ftbd_prefix_silent_sublist: forall l p, ftbd_prefix l (list_to_silent_trace p) -> list_pref l p.
-Proof.
-  induction l; intros p Hpref; auto.
-  destruct p; inversion Hpref.
-  subst. simpl. split; auto.
-Qed.
+(* Lemma ftbd_prefix_silent_sublist: forall l p, ftbd_prefix l (list_to_silent_trace p) -> list_pref l p. *)
+(* Proof. *)
+(*   induction l; intros p Hpref; auto. *)
+(*   destruct p; inversion Hpref. *)
+(*   subst. simpl. split; auto. *)
+(* Qed. *)
 
-Lemma snocs_same_continuation: forall (l p : list event) e1 e2,
-    list_pref (snoc l e1) p -> list_pref (snoc l e2) p -> e1 = e2. 
-Proof.
-  induction l; intros [] e1 e2 H1 H2; inversion H1; inversion H2; subst; auto.  
-  now apply (IHl l0 e1 e2).   
-Qed. 
+(* Lemma snocs_same_continuation: forall (l p : list event) e1 e2, *)
+(*     list_pref (snoc l e1) p -> list_pref (snoc l e2) p -> e1 = e2.  *)
+(* Proof. *)
+(*   induction l; intros [] e1 e2 H1 H2; inversion H1; inversion H2; subst; auto.   *)
+(*   now apply (IHl l0 e1 e2).    *)
+(* Qed.  *)
 
-Lemma snocs_aux_lemma: forall (l p : list event) i1 i2 a,
-    i1 <> i2 -> list_pref (snoc l i1) (snoc p a) -> list_pref (snoc l i2) p -> False.
-Proof.
-  induction l; intros [] i1 i2 ev Hdiff Hpref1 Hpref2;
-    inversion Hpref1; inversion Hpref2; subst.
-  + now apply Hdiff. 
-  + now apply (IHl l0 i1 i2 ev).     
-Qed.
+(* Lemma snocs_aux_lemma: forall (l p : list event) i1 i2 a, *)
+(*     i1 <> i2 -> list_pref (snoc l i1) (snoc p a) -> list_pref (snoc l i2) p -> False. *)
+(* Proof. *)
+(*   induction l; intros [] i1 i2 ev Hdiff Hpref1 Hpref2; *)
+(*     inversion Hpref1; inversion Hpref2; subst. *)
+(*   + now apply Hdiff.  *)
+(*   + now apply (IHl l0 i1 i2 ev).      *)
+(* Qed. *)
 
 (*********************************************************************************)
 
 Definition myXr (x1 x2: xpref) : Prop :=
   (xpr x1 x2) \/ (xpr x2 x1) \/
-  (exists p i1 i2, is_input i1 /\
+  (exists l i1 i2, is_input i1 /\
                is_input i2 /\
                i1 <> i2 /\
-               xpr (xtbd (snoc p i1)) x1 /\
-               xpr (xtbd (snoc p i2)) x2).
+               xpr (xtbd (snoc l i1)) x1 /\
+               xpr (xtbd (snoc l i2)) x2).
 
 
+Lemma myXr_symmetric : forall x1 x2, myXr x1 x2 -> myXr x2 x1.
+ Proof. firstorder. Qed. 
+
+Lemma auXiliary_tstop :
+  forall x2 l1 e1 t2, xprefix x2 t2 ->
+                  traces_match (tstop l1 e1) t2 -> myXr (xstop l1 e1) x2.
+Proof.
+  intros x2 l1 e1 t2 xprefix2 [Heq | [ll [i1 [i2 [I1 [I2 [Idiff [l_prefix1 l_prefix2]]]]]]]].
+  + rewrite <- Heq in *. destruct (xsame_ext (xstop l1 e1) x2 (tstop l1 e1)); simpl; auto;
+                          [now left |  right; now left].
+  + destruct x2, t2; simpl in xprefix2; simpl in l_prefix1, l_prefix2; try now auto.   
+    ++ inversion xprefix2; subst.  
+       right. right. now exists ll, i1, i2.
+    ++ destruct (list_list_same_ext l ll l0); auto.
+       apply (list_list_prefix_trans ll (snoc ll i2) l0); auto.
+       now apply snoc_longer.
+       +++ right. left. simpl. apply (list_list_prefix_trans l (snoc ll i1) l1); auto.
+           apply (list_list_prefix_trans l ll _ ); auto. now apply snoc_longer.
+       +++ admit. (* contradiction! *)
+    ++ destruct (list_list_same_ext l ll l0); auto.
+       apply (list_list_prefix_trans ll (snoc ll i2) l0); auto.
+       now apply snoc_longer.
+       +++ right. left. simpl. apply (list_list_prefix_trans l (snoc ll i1) l1); auto.
+           apply (list_list_prefix_trans l ll _ ); auto. now apply snoc_longer.
+       +++ admit.
+    ++ destruct (list_stream_same_ext l ll s); auto.
+       apply (list_stream_prefix_trans ll (snoc ll i2) s); auto.
+       now apply snoc_longer.
+       +++ right. left. simpl. apply (list_list_prefix_trans l (snoc ll i1) l1); auto.
+           apply (list_list_prefix_trans l ll _ ); auto. now apply snoc_longer.
+       +++ admit. 
+Admitted.
+
+Lemma auXiliary_tsilent :
+  forall x2 l1 t2, xprefix x2 t2 ->
+                traces_match (tsilent l1) t2 -> myXr (xsilent l1) x2.
+Proof.
+  intros x2 l1 t2 xprefix2 [Heq | [ll [i1 [i2 [I1 [I2 [Idiff [l_prefix1 l_prefix2]]]]]]]].
+  + rewrite <- Heq in *. destruct (xsame_ext (xsilent l1) x2 (tsilent l1)); simpl; auto;
+                          [now left |  right; now left].
+  + destruct x2, t2; simpl in xprefix2; simpl in l_prefix1, l_prefix2; try now auto.   
+    ++ inversion xprefix2; subst.  
+       right. right. now exists ll, i1, i2.
+    ++ destruct (list_list_same_ext l ll l0); auto.
+       apply (list_list_prefix_trans ll (snoc ll i2) l0); auto.
+       now apply snoc_longer.
+       +++ right. left. simpl. apply (list_list_prefix_trans l (snoc ll i1) l1); auto.
+           apply (list_list_prefix_trans l ll _ ); auto. now apply snoc_longer.
+       +++ admit. (* contradiction! *)
+    ++ destruct (list_list_same_ext l ll l0); auto.
+       apply (list_list_prefix_trans ll (snoc ll i2) l0); auto.
+       now apply snoc_longer.
+       +++ right. left. simpl. apply (list_list_prefix_trans l (snoc ll i1) l1); auto.
+           apply (list_list_prefix_trans l ll _ ); auto. now apply snoc_longer.
+       +++ admit.
+    ++ destruct (list_stream_same_ext l ll s); auto.
+       apply (list_stream_prefix_trans ll (snoc ll i2) s); auto.
+       now apply snoc_longer.
+       +++ right. left. simpl. apply (list_list_prefix_trans l (snoc ll i1) l1); auto.
+           apply (list_list_prefix_trans l ll _ ); auto. now apply snoc_longer.
+       +++ admit. 
+Admitted.
+
+
+Lemma auXiliary_lemma:
+  forall x1 x2 t1 t2, xprefix x1 t1 -> xprefix x2 t2 -> traces_match t1 t2 -> myXr x1 x2.
+Proof.
+  intros x1 x2 t1 t2 xprefix1 xprefix2 [Heq | [ll [i1 [i2 [I1 [I2 [Idiff [l_prefix1 l_prefix2]]]]]]]]. 
+  - subst. unfold myXr. destruct (xsame_ext x1 x2 t2) as [go_left | go_right_left]; auto. 
+  - destruct x1, x2.
+    ++ destruct t1, t2; inversion xprefix1; inversion xprefix2; subst.
+       right. right. now exists ll, i1, i2.
+    ++ destruct t1; inversion xprefix1; subst.  
+       apply (auXiliary_tstop (xtbd l0) l1 e0 t2); auto.
+       right. now exists ll, i1, i2. 
+    ++ destruct t1, t2; inversion xprefix1; inversion xprefix2; subst.
+       simpl in *. right. right. now exists ll, i1, i2.
+    ++ destruct t2; inversion xprefix2; subst. apply myXr_symmetric. 
+       apply (auXiliary_tstop (xtbd l) l1 e0 t1); auto.
+       right. exists ll, i2, i1. repeat (split; try now auto). 
+    ++ admit.   
+    ++ admit. 
+    ++ destruct t1, t2; inversion xprefix1; inversion xprefix2; subst.
+       simpl in *. right. right. now exists ll, i1, i2.
+    ++ admit.
+    ++ destruct t1, t2; inversion xprefix1; inversion xprefix2; subst.
+       simpl in *. right. right. now exists ll, i1, i2.  
+ 
 Lemma teq_premises_myXr_holds : forall P1 P2,
     (forall Cs t, sem src (Cs [P1]) t <-> sem src (Cs [P2]) t) ->
     (forall Cs x1 x2, xsem (Cs [P1]) x1 -> xsem (Cs [P2]) x2 ->
                  myXr x1 x2).
 Proof.
   intros P1 P2 H Cs x1 x2 [t1 [xpref1 sem1]] [t2 [xpref2 sem2]].
+    rewrite (H Cs t1) in sem1.
+   specialize (determinacy_src (Cs[P2]) t1 t2 sem1 sem2). 
+   intros Hmatch. now apply (auXiliary_lemma x1 x2 t1 t2).
+Qed.
+
+   destruct (determinacy_src (Cs[P2]) t1 t2 sem1 sem2) as [t_eq | matching]; try now auto.  
+  + subst.  destruct (xsame_ext _ _ _ xpref1 xpref2) as  [go_left | go_right];
+      [now left | right; now left].
+  + destruct matching as [ll [i1 [i2 [I1 [I2 [Idiff [l_prefix1 l_prefix2]]]]]]].
+    destruct t1, t2; inversion xpref1; inversion xpref2; subst.
+    simpl in *. right. right. now exists ll, i1, i2.
+  + subst.  destruct (xsame_ext _ _ _ xpref1 xpref2) as  [go_left | go_right];
+              [now left | right; now left].
+  + apply 
+    destruct matching as [ll [i1 [i2 [I1 [I2 [Idiff [l_prefix1 l_prefix2]]]]]]].
+    destruct t1, t2; inversion xpref1; subst. 
+    ++ simpl in *. 
+    
+    apply list_proper_or_equal in xpref2. destruct xpref2 as [K | [a K]].
+    subst.
+     ++ right. right. now exists ll, i1, i2.
+     ++ destruct (list_list_same_ext (snoc ll i2) (snoc l0 a) l2) as [F | F]; auto.
+        * 
+        * apply list_pref_snoc_pref in F. right. left.
+          simpl. apply (list_list_prefix_trans l0 ll l1); auto.
+          apply (list_list_prefix_trans ll (snoc ll i1) l1); auto.
+          now apply snoc_longer.
+     ++  
+
+    
+  + inversion xpref1; inversion xpref2; subst.
+    destruct (determinacy_src (Cs[P2]) (tstop l1 e1) (tstop l2 e2) sem1 sem2) as [t_eq | matching]. 
+  + admit. 
+  
+  + destruct t1, t2; inversion xpref1; inversion xpref2; subst; auto. 
+    rewrite (H Cs (tstop l1 e1)) in sem1.
+    destruct (determinacy_src (Cs[P2]) (tstop l1 e1) (tstop l2 e2) sem1 sem2) as [t_eq | matching].
+    ++ rewrite t_eq in *.
+    destruct (xsame_ext _ _ _ xpref1 xpref2) as  [go_left | go_right];
+      [now left | right; now left].
+    ++ destruct matching as [l [i1 [i2 [I1 [I2 [Idiff [l_prefix1 l_prefix2]]]]]]].
+       simpl in l_prefix1, l_prefix2.
+       right. right. exists l, i1, i2. repeat (split; try now auto).
+  +  destruct t1, t2; inversion xpref1; subst; auto.
+     rewrite (H Cs (tstop l1 e0)) in sem1.
+     destruct (determinacy_src (Cs[P2]) (tstop l1 e0) (tstop l2 e1) sem1 sem2) as [t_eq | matching].
+     inversion t_eq; subst. simpl in xpref2. right. left. now simpl. 
+     destruct matching as [l [i1 [i2 [I1 [I2 [Idiff [l_prefix1 l_prefix2]]]]]]].
+     simpl in *.
+     
+
+     
+  intros P1 P2 H Cs x1 x2 [t1 [xpref1 sem1]] [t2 [xpref2 sem2]].
   rewrite (H Cs t1) in sem1.
   destruct (determinacy_src (Cs[P2]) t1 t2 sem1 sem2) as [t_eq | matching].
   + rewrite t_eq in *.
-    destruct (same_x_ext x1 x2 t2 xpref1 xpref2) as  [go_left | go_right];
+    destruct (xsame_ext x1 x2 t2 xpref1 xpref2) as  [go_left | go_right];
       [now left | right; now left].
-  + destruct matching as [m [i1 [i2 [I1 [I2 [Idiff [m_stop [m_prefix1 m_prefix2]]]]]]]].
-    destruct m.
-    ++ inversion m_stop.
-    ++ simpl in m_prefix1, m_prefix2.
+  + destruct matching as [l [i1 [i2 [I1 [I2 [Idiff [l_prefix1 l_prefix2]]]]]]].
+    destruct l. 
+    ++ simpl in l_prefix1, l_prefix2.
        destruct x1, x2.
        - apply unique_continuation_stop in xpref1.
          apply unique_continuation_stop in xpref2.
